\documentclass[letterpaper,11pt]{article}
\usepackage{amssymb, amsmath}
\usepackage[hmargin=1in,vmargin=1in]{geometry}
\begin{document}
\textbf{08.24} \\
Let $Y _{n} \sim \chi ^2(n)$. Find the limiting distribution of $(Y _{n}-n)/ \sqrt{2n}$ as n $\rightarrow \infty$, using moment generating functions. 
\vspace{0.25in}\\ 
First, note that the MGF of $Y_{n}$ is $M_{Y_{n}} = \Big( \frac{1} {1-2t} \Big) ^{n/2}$. Then,\\

$M_{\frac{(Y_{n}-n)}{\sqrt{2n}}} (t)
= E\Big[e^{t \frac{(Y_{n}-n)} {\sqrt{2n}} } \Big] 
= E\Big[e^{\big( \frac{t} {\sqrt{2n}}Y_{n} \big)} e^{\big( \frac{-tn} {\sqrt{2n}} \big)} \Big]
= e^{\frac{-tn} {\sqrt{2n}} } E\Big[e^{\big( \frac{t} {\sqrt{2n}}Y_{n} \big)} \Big]  
\vspace{1mm}\\$

$\hspace{0.75in}
= e^{\frac{-tn} {\sqrt{2n}} } M_{Y_{n}} \Big( \frac{t} {\sqrt{2n}} \Big)
= e^{ \frac{-tn} {\sqrt{2n}} } \Bigg( \frac{1} {1-2 \big( \frac{t} {\sqrt{2n}} \big) } \Bigg) ^{n/2}
= e^{ \frac{-tn} {\sqrt{2n}} } \bigg( \frac{ \sqrt{2n}} { \sqrt{2n} - 2t} \bigg) ^{n/2} 
\vspace{1mm} $\\ 

$\hspace{0.75in}
= e^{ \frac{-tn} {\sqrt{2n}} } \bigg( 1- \frac {2t} {\sqrt{2n}} \bigg) ^{-n/2} 
= e^{ -t \sqrt{n/2} } \bigg( 1- t \sqrt{2/n} \bigg) ^{-n/2}
\vspace{10mm} \\ $
Next we take the limit. \\ 

$\displaystyle \lim_{n\to\infty}M_{\frac{(Y_{n}-n)}{\sqrt{2n}}} (t) 
= \displaystyle \lim_{n\to\infty} e^{-t \sqrt{n/2}} (1-t \sqrt{2/n})^{-n/2}
\vspace{1mm} \\$

$\hspace{1.1in}
=\displaystyle \lim_{m\to\infty} e^{-tm} (1-t/m)^{-m^2}
\hspace{2.5in}
$Let $m=\sqrt{n/2} $\\ 

$ \ln \displaystyle \lim_{n\to\infty} M_{\frac{(Y_{n}-n)}{\sqrt{2n}}} (t)
= \displaystyle \lim_{m\to\infty} \ln \Big( e^{-tm} (1-t/m)^{-m^2} \Big)
\hspace{2in}
$Log both sides$
\vspace{1mm} $\\

$\hspace{1.1in}
= \displaystyle \lim_{m\to\infty} \Big( -tm -m^2 \ln(1-t/m) \Big) 
\vspace{1mm} $\\

$\hspace{1.1in} 
= -\displaystyle \lim_{m\to\infty} \Big( m^2 (t/m + \ln(1-t/m) \Big)
\vspace{1mm} $\\

$\hspace{1.1in}
= -\displaystyle \lim_{x\to 0^+} \Bigg( \frac {tx + \ln(1-tx)} {x^2} \Bigg)
\hspace{2.5in}
$Let $ x=1/m 
\vspace{1mm} $\\

$\hspace{1.1in} 
=- \displaystyle \lim_{x\to 0^+} \Bigg( \frac {t - \frac{t} {(1-tx)}} {2x} \Bigg)
\hspace{2.25in}
$Use L'Hospital's Rule$ 
\vspace{1mm} $\\

$\hspace{1.1in} 
= -\frac{t} {2} \displaystyle \lim_{x\to 0^+} \Bigg( \frac {\frac{-tx} {(1-tx)}} {x} \Bigg)
\vspace{1mm} $\\

$\hspace{1.1in} 
= \frac{t^2} {2} \displaystyle \lim_{x\to 0^+} \Big( \frac {1} {1-tx} \Big)
\vspace{1mm} $\\

$\hspace{1.1in} 
=t^2/2
\vspace{10mm}$\\
Hence, $\displaystyle \lim_{n\to\infty}M_{\frac{(Y_{n}-n)}{\sqrt{2n}}} (t) = e^{t^2/2}$ which is the MGF of the random variable for the standard normal distribution. 

\end{document}
